Clean/Examples/Add32Explicit.lean
@@ -23,6 +23,8 @@ example : ExplicitCircuit.output (circuit32 default) 0
 
 example : ((circuit32 default).operations 0).SubcircuitsConsistent 0 :=
   ExplicitCircuits.subcircuitsConsistent ..
+example : ((circuit32 default).operations 0).SubcircuitsLawful :=
+  ExplicitCircuits.subcircuitsLawful _ _
 
 example (x0 x1 x2 x3 y0 y1 y2 y3 carryIn : Expression (F pBabybear)) env (i0 : ℕ) :
   Circuit.ConstraintsHold.Soundness env ((circuit32 ⟨ ⟨ x0, x1, x2, x3 ⟩, ⟨ y0, y1, y2, y3 ⟩, carryIn ⟩).operations i0)
