Clean/Gadgets/Rotation64/Rotation64Bytes.lean
@@ -51,6 +51,9 @@ instance elaborated (off : Fin 8): ElaboratedCircuit (F p) U64 U64 where
   subcircuitsConsistent x i0 := by
     simp only [main]
     fin_cases off <;> simp only [circuit_norm, reduceIte, Fin.reduceFinMk, Fin.reduceEq]
+  subcircuitsLawful _ _ := by
+    simp only [main]
+    fin_cases off <;> simp only [circuit_norm, reduceIte, Fin.reduceFinMk, Fin.reduceEq]
 
   output_eq := by
     intros
